Construct NFS error codes from Dafny
Implementing this change somehow broke all the proofs, we we also
restructured the invariant to make it much more local and better
triggered.

There are a handful more postconditions for error cases but we might be
able to extend these.

nfsd/ops.go
@@ -6,9 +6,11 @@ import (
 	direntries "github.com/mit-pdos/dafny-jrnl/dafnygen/DirEntries_Compile"
 	dirfs "github.com/mit-pdos/dafny-jrnl/dafnygen/DirFs_Compile"
 	inode "github.com/mit-pdos/dafny-jrnl/dafnygen/Inode_Compile"
+	_dafny "github.com/mit-pdos/dafny-jrnl/dafnygen/dafny"
 	dafny "github.com/mit-pdos/dafny-jrnl/dafnygen/dafny"
 
 	"github.com/mit-pdos/dafny-jrnl/dafny_go/bytes"
+	"github.com/mit-pdos/dafny-jrnl/dafny_go/jrnl"
 
 	"github.com/mit-pdos/goose-nfsd/nfstypes"
 	"github.com/mit-pdos/goose-nfsd/util"
@@ -25,35 +27,39 @@ func (nfs *Nfs) NFSPROC3_NULL() {
 	util.DPrintf(0, "NFS Null\n")
 }
 
+func (nfs *Nfs) runTxn(f func(txn *jrnl.Txn) dirfs.Result) (v interface{}, status nfstypes.Nfsstat3) {
+	txn := nfs.filesys.Begin()
+	r := f(txn)
+	var statusCode uint32
+	v, statusCode = dirfs.Companion_Default___.HandleResult(r, txn)
+	status = nfstypes.Nfsstat3(statusCode)
+	return
+}
+
 func (nfs *Nfs) NFSPROC3_GETATTR(args nfstypes.GETATTR3args) nfstypes.GETATTR3res {
 	var reply nfstypes.GETATTR3res
 	util.DPrintf(1, "NFS GetAttr %v\n", args)
 
-	txn := nfs.filesys.Begin()
 	inum := fh2ino(args.Object)
 
-	ok, stat := nfs.filesys.GETATTR(txn, inum)
-	if ok {
-		ok = txn.Commit()
-	} else {
-		txn.Abort()
+	stat, status := nfs.runTxn(func(txn *jrnl.Txn) dirfs.Result {
+		return nfs.filesys.GETATTR(txn, inum)
+	})
+	reply.Status = status
+	if status != nfstypes.NFS3_OK {
+		return reply
 	}
 
-	if ok {
-		attrs := stat.Get().(dirfs.Attributes_Attributes)
-		if attrs.Is__dir {
-			reply.Resok.Obj_attributes.Ftype = nfstypes.NF3DIR
-		} else {
-			reply.Resok.Obj_attributes.Ftype = nfstypes.NF3REG
-		}
-		reply.Resok.Obj_attributes.Mode = 0777
-		reply.Resok.Obj_attributes.Nlink = 1
-		reply.Resok.Obj_attributes.Size = nfstypes.Size3(attrs.Size)
-		reply.Resok.Obj_attributes.Fileid = nfstypes.Fileid3(inum)
-		reply.Status = nfstypes.NFS3_OK
+	attrs := stat.(dirfs.Attributes).Get().(dirfs.Attributes_Attributes)
+	if attrs.Is__dir {
+		reply.Resok.Obj_attributes.Ftype = nfstypes.NF3DIR
 	} else {
-		reply.Status = nfstypes.NFS3ERR_SERVERFAULT
+		reply.Resok.Obj_attributes.Ftype = nfstypes.NF3REG
 	}
+	reply.Resok.Obj_attributes.Mode = 0777
+	reply.Resok.Obj_attributes.Nlink = 1
+	reply.Resok.Obj_attributes.Size = nfstypes.Size3(attrs.Size)
+	reply.Resok.Obj_attributes.Fileid = nfstypes.Fileid3(inum)
 
 	return reply
 }
@@ -71,25 +77,18 @@ func (nfs *Nfs) NFSPROC3_LOOKUP(args nfstypes.LOOKUP3args) nfstypes.LOOKUP3res {
 	util.DPrintf(1, "NFS Lookup %v\n", args)
 	var reply nfstypes.LOOKUP3res
 
-	txn := nfs.filesys.Begin()
 	inum := fh2ino(args.What.Dir)
 	name := seqOfString(args.What.Name)
 
-	err, found, f_ino := nfs.filesys.LOOKUP(txn, inum, name)
-	if !err.Is_NoError() {
-		txn.Abort()
-		reply.Status = nfstypes.NFS3ERR_SERVERFAULT
+	f_ino, status := nfs.runTxn(func(txn *jrnl.Txn) dirfs.Result {
+		return nfs.filesys.LOOKUP(txn, inum, name)
+	})
+	reply.Status = status
+	if status != nfstypes.NFS3_OK {
 		return reply
 	}
-	if !found {
-		txn.Commit()
-		reply.Status = nfstypes.NFS3ERR_NOENT
-		return reply
-	}
-	fh := Fh{Ino: f_ino}
+	fh := Fh{Ino: f_ino.(uint64)}
 	reply.Resok.Object = fh.MakeFh3()
-	reply.Status = nfstypes.NFS3_OK
-	txn.Commit()
 	return reply
 }
 
@@ -105,23 +104,22 @@ func (nfs *Nfs) NFSPROC3_READ(args nfstypes.READ3args) nfstypes.READ3res {
 	var reply nfstypes.READ3res
 	util.DPrintf(1, "NFS Read %v %d %d\n", args.File, args.Offset, args.Count)
 
-	txn := nfs.filesys.Begin()
 	inum := fh2ino(args.File)
+	off := uint64(args.Offset)
+	count := uint64(args.Count)
 
-	// args.Offset
-	// args.Count
-	err, bs := nfs.filesys.READ(txn, inum, uint64(args.Offset), uint64(args.Count))
-	if !err.Is_NoError() {
-		reply.Status = nfstypes.NFS3ERR_NOTSUPP
-		txn.Abort()
+	r, status := nfs.runTxn(func(txn *jrnl.Txn) dirfs.Result {
+		return nfs.filesys.READ(txn, inum, off, count)
+	})
+	reply.Status = status
+	if status != nfstypes.NFS3_OK {
 		return reply
 	}
+	bs := r.(*bytes.Bytes)
 
 	reply.Resok.Count = nfstypes.Count3(bs.Len())
 	reply.Resok.Data = bs.Data
 	reply.Resok.Eof = false
-	reply.Status = nfstypes.NFS3_OK
-	txn.Commit()
 	return reply
 }
 
@@ -130,23 +128,21 @@ func (nfs *Nfs) NFSPROC3_WRITE(args nfstypes.WRITE3args) nfstypes.WRITE3res {
 	util.DPrintf(1, "NFS Write %v off %d cnt %d how %d\n", args.File, args.Offset,
 		args.Count, args.Stable)
 
-	txn := nfs.filesys.Begin()
 	inum := fh2ino(args.File)
 
 	// XXX write at offset args.Offset
 
 	bs := bytes.Data(args.Data)
-	err := nfs.filesys.Append(txn, inum, bs)
-	if !err.Is_NoError() {
-		reply.Status = nfstypes.NFS3ERR_NOTSUPP
-		txn.Abort()
+	_, status := nfs.runTxn(func(txn *jrnl.Txn) dirfs.Result {
+		return nfs.filesys.Append(txn, inum, bs)
+	})
+	reply.Status = status
+	if status != nfstypes.NFS3_OK {
 		return reply
 	}
 
 	reply.Resok.Count = args.Count
 	reply.Resok.Committed = nfstypes.FILE_SYNC
-	reply.Status = nfstypes.NFS3_OK
-	txn.Commit()
 	return reply
 }
 
@@ -172,21 +168,20 @@ func (nfs *Nfs) NFSPROC3_CREATE(args nfstypes.CREATE3args) nfstypes.CREATE3res {
 	util.DPrintf(1, "NFS Create %v\n", args)
 	var reply nfstypes.CREATE3res
 
-	txn := nfs.filesys.Begin()
 	inum := fh2ino(args.Where.Dir)
 
 	nameseq := seqOfString(args.Where.Name)
-	ok, finum := nfs.filesys.CREATE(txn, inum, nameseq)
-	if !ok {
-		reply.Status = nfstypes.NFS3ERR_NOTSUPP
-		txn.Abort()
+	r, status := nfs.runTxn(func(txn *jrnl.Txn) dirfs.Result {
+		return nfs.filesys.CREATE(txn, inum, nameseq)
+	})
+	reply.Status = status
+	if status != nfstypes.NFS3_OK {
 		return reply
 	}
+	finum := r.(uint64)
 
 	// XXX set size based on args.How.Obj_attributes.Size
 
-	txn.Commit()
-	reply.Status = nfstypes.NFS3_OK
 	reply.Resok.Obj.Handle_follows = true
 	reply.Resok.Obj.Handle = Fh{Ino: finum}.MakeFh3()
 	return reply
@@ -196,19 +191,19 @@ func (nfs *Nfs) NFSPROC3_MKDIR(args nfstypes.MKDIR3args) nfstypes.MKDIR3res {
 	util.DPrintf(1, "NFS Mkdir %v\n", args)
 	var reply nfstypes.MKDIR3res
 
-	txn := nfs.filesys.Begin()
 	inum := fh2ino(args.Where.Dir)
 
 	nameseq := seqOfString(args.Where.Name)
-	ok, finum := nfs.filesys.MKDIR(txn, inum, nameseq)
-	if !ok {
-		reply.Status = nfstypes.NFS3ERR_NOTSUPP
-		txn.Abort()
+
+	r, status := nfs.runTxn(func(txn *jrnl.Txn) dirfs.Result {
+		return nfs.filesys.MKDIR(txn, inum, nameseq)
+	})
+	reply.Status = status
+	if status != nfstypes.NFS3_OK {
 		return reply
 	}
+	finum := r.(uint64)
 
-	txn.Commit()
-	reply.Status = nfstypes.NFS3_OK
 	reply.Resok.Obj.Handle_follows = true
 	reply.Resok.Obj.Handle = Fh{Ino: finum}.MakeFh3()
 	return reply
@@ -239,18 +234,17 @@ func (nfs *Nfs) NFSPROC3_REMOVE(args nfstypes.REMOVE3args) nfstypes.REMOVE3res {
 	util.DPrintf(1, "NFS Remove %v\n", args)
 	var reply nfstypes.REMOVE3res
 
-	txn := nfs.filesys.Begin()
 	inum := fh2ino(args.Object.Dir)
 	name := seqOfString(args.Object.Name)
-	err := nfs.filesys.REMOVE(txn, inum, name)
-	if !err.Is_NoError() {
-		// XXX do better job conveying errors, EINVAL for !dir
-		reply.Status = nfstypes.NFS3ERR_NOENT
-		txn.Abort()
+
+	_, status := nfs.runTxn(func(txn *jrnl.Txn) dirfs.Result {
+		return nfs.filesys.REMOVE(txn, inum, name)
+	})
+	reply.Status = status
+	if status != nfstypes.NFS3_OK {
 		return reply
 	}
-	reply.Status = nfstypes.NFS3_OK
-	txn.Commit()
+
 	return reply
 }
 
@@ -279,15 +273,16 @@ func (nfs *Nfs) NFSPROC3_READDIR(args nfstypes.READDIR3args) nfstypes.READDIR3re
 	util.DPrintf(1, "NFS Readdir %v\n", args)
 	var reply nfstypes.READDIR3res
 
-	txn := nfs.filesys.Begin()
 	inum := fh2ino(args.Dir)
 
-	err, seq := nfs.filesys.READDIR(txn, inum)
-	if !err.Is_NoError() {
-		txn.Abort()
-		reply.Status = nfstypes.NFS3ERR_SERVERFAULT
+	r, status := nfs.runTxn(func(txn *jrnl.Txn) dirfs.Result {
+		return nfs.filesys.READDIR(txn, inum)
+	})
+	reply.Status = status
+	if status != nfstypes.NFS3_OK {
 		return reply
 	}
+	seq := r.(_dafny.Seq)
 
 	seqlen := seq.LenInt()
 	var ents *nfstypes.Entry3
@@ -306,8 +301,6 @@ func (nfs *Nfs) NFSPROC3_READDIR(args nfstypes.READDIR3args) nfstypes.READDIR3re
 		}
 	}
 
-	txn.Commit()
-	reply.Status = nfstypes.NFS3_OK
 	reply.Resok.Reply = nfstypes.Dirlist3{Entries: ents, Eof: true}
 	return reply
 }
